high2/Zeta.High.Verifier.EAC.fst
@@ -1,17 +1,62 @@
 module Zeta.High.Verifier.EAC
 
+open Zeta.App
+open Zeta.Key
+open Zeta.GenericVerifier
+open Zeta.EAC
 open Zeta.High.Interleave
 
+module I = Zeta.Interleave
 module GI=Zeta.Generic.Interleave
 module GTL=Zeta.Generic.TSLog
 module HI=Zeta.High.Interleave
 module HTL=Zeta.High.TSLog
+module IF=Zeta.IdxFn
+
+type failure_info (app:app_params) (n:nat) = {
+  bi: nat;
+  bk: base_key;
+  es: eac_state app bk;
+  le: vlog_entry app
+}
+
+let eac_failure (#app #n:_) (il: neac_log app n)
+  : failure_info app n
+  = let bi = eac_boundary il in
+    let bk = eac_fail_key il in
+    let es = IF.to_pre_fn (eac_state_of_key bk) il bi in
+    let le = I.index il bi in
+    { bi; bk; es; le}
+
+let lemma_non_eac_init_addb
+  (#app #n:_)
+  (epmax: epoch)
+  (itsl: neac_before_epoch app n epmax
+    {let fi = eac_failure itsl in
+     GI.aems_equal_upto epmax itsl /\
+     fi.es = EACInit /\
+     AddB? fi.le})
+  = let fi = eac_failure itsl in
+    let e = I.prefix itsl fi.bi in
+    //let be = blum_add_elem itsl fi.bi in
+
+    admit()
 
 let lemma_neac_implies_hash_collision
   (#app #n:_)
   (epmax: epoch)
   (itsl: neac_before_epoch app n epmax {GI.aems_equal_upto epmax itsl})
   : hash_collision app
-  = let i = HI.eac_boundary itsl in
+  = let fi = eac_failure itsl in
     eac_boundary_not_appfn itsl;
+
+    match fi.es with
+    | EACInit -> (
+      match fi.le with
+      | AddB _ _ _ _ -> lemma_non_eac_init_addb epmax itsl
+      | _ ->
+      admit()
+    )
+    | _ ->
+
     admit()
